compiler/src/FlatToRiscvBitWidthSpecifics.v
@@ -1,7 +1,0 @@
-Require Import coqutil.Map.Interface.
-Require Import riscv.util.BitWidths.
-Require Import riscv.Memory.
-
-Class FlatToRiscvBitWidthSpecifics{byte: Type}(mword: Type){Mem: map.map mword byte} := {
-  BitWidth: BitWidths;
-}.
