compiler/src/FlattenExpr.v
@@ -6,7 +6,6 @@ Require compiler.FlatImp.
 Require Import compiler.NameGen.
 Require Import bbv.DepEqNat.
 Require Import coqutil.Decidable.
-Require Import riscv.util.BitWidths.
 Require Import riscv.Memory.
 Require Import riscv.Utility.
 Require Import bedrock2.Syntax.
