compiler/src/examples/CompileExamples.v
@@ -9,9 +9,6 @@ Require Import compiler.ExprImp.
 Require Import compiler.NameGen.
 Require Import compiler.Pipeline.
 Require Import compiler.util.Common.
-Require Import riscv.util.BitWidths.
-Require Import riscv.util.BitWidth32.
-Require Import compiler.FlatToRiscv32Specifics.
 Require Import coqutil.Map.SortedList.
 Require Import compiler.ZNameGen.
 Require Import riscv.InstructionCoercions.
